Pedro-Coq/proofs/SlideKickDustExecution.v
@@ -1,0 +1,306 @@
+From Coq Require Import Lia List ZArith.
+From compcert Require Import AST Clight Clightdefs ClightBigstep Cop Ctypes
+  Errors Events Floats Globalenvs Integers Maps Memory Values.
+From Pedro.Generated Require Import
+  us_mario_actions_moving jp_mario_actions_moving
+  us_mario jp_mario us_mario_step jp_mario_step
+  us_audio_external jp_audio_external.
+From Pedro.Proofs Require Import GameTypes ASTFacts TTCCogExecution.
+
+Import ListNotations.
+Open Scope Z_scope.
+Module SK := us_mario_actions_moving.
+
+(** This is a caller execution, not a reachable cog-Pedro witness. The seven
+    helper executions below are residuals over the actual generated functions.
+    In particular, the real collision query, sliding update, animation state,
+    and complete frame still have to be supplied. No helper is replaced by a
+    newly invented implementation. *)
+Definition slide_kick_function (version : GameVersion) : function :=
+  match version with
+  | VersionUS => SK.f_act_slide_kick_slide
+  | VersionJP => jp_mario_actions_moving.f_act_slide_kick_slide
+  end.
+
+Definition slide_animation_function (version : GameVersion) : function :=
+  match version with VersionUS => us_mario.f_set_mario_animation
+                   | VersionJP => jp_mario.f_set_mario_animation end.
+Definition slide_animation_end_function (version : GameVersion) : function :=
+  match version with VersionUS => us_mario.f_is_anim_at_end
+                   | VersionJP => jp_mario.f_is_anim_at_end end.
+Definition slide_update_function (version : GameVersion) : function :=
+  match version with VersionUS => SK.f_update_sliding
+                   | VersionJP => jp_mario_actions_moving.f_update_sliding end.
+Definition slide_ground_function (version : GameVersion) : function :=
+  match version with VersionUS => us_mario_step.f_perform_ground_step
+                   | VersionJP => jp_mario_step.f_perform_ground_step end.
+Definition slide_reflection_function (version : GameVersion) : function :=
+  match version with VersionUS => us_mario_step.f_mario_bonk_reflection
+                   | VersionJP => jp_mario_step.f_mario_bonk_reflection end.
+Definition slide_action_function (version : GameVersion) : function :=
+  match version with VersionUS => us_mario.f_set_mario_action
+                   | VersionJP => jp_mario.f_set_mario_action end.
+Definition slide_sound_function (version : GameVersion) : function :=
+  match version with VersionUS => us_audio_external.f_play_sound
+                   | VersionJP => jp_audio_external.f_play_sound end.
+
+Theorem slide_kick_caller_identical_us_jp :
+  SK.f_act_slide_kick_slide =
+    jp_mario_actions_moving.f_act_slide_kick_slide.
+Proof. reflexivity. Qed.
+
+Record slide_caller_layout (ge : Clight.genv) : Type := {
+  slide_mario_co : composite;
+  slide_object_co : composite;
+  slide_node_co : composite;
+  slide_gfx_co : composite;
+  slide_mario_layout : (genv_cenv ge) ! SK._MarioState = Some slide_mario_co;
+  slide_input_offset : field_offset (genv_cenv ge) SK._input
+    (co_members slide_mario_co) = OK (2, Full);
+  slide_particles_offset : field_offset (genv_cenv ge) SK._particleFlags
+    (co_members slide_mario_co) = OK (8, Full);
+  slide_terrain_offset : field_offset (genv_cenv ge) SK._terrainSoundAddend
+    (co_members slide_mario_co) = OK (20, Full);
+  slide_object_offset : field_offset (genv_cenv ge) SK._marioObj
+    (co_members slide_mario_co) = OK (136, Full);
+  slide_position_offset : field_offset (genv_cenv ge) SK._pos
+    (co_members slide_mario_co) = OK (60, Full);
+  slide_floor_offset : field_offset (genv_cenv ge) SK._floor
+    (co_members slide_mario_co) = OK (104, Full);
+  slide_floor_height_offset : field_offset (genv_cenv ge) SK._floorHeight
+    (co_members slide_mario_co) = OK (112, Full);
+  slide_object_layout : (genv_cenv ge) ! SK._Object = Some slide_object_co;
+  slide_header_offset : field_offset (genv_cenv ge) SK._header
+    (co_members slide_object_co) = OK (0, Full);
+  slide_node_layout : (genv_cenv ge) ! SK._ObjectNode = Some slide_node_co;
+  slide_gfx_offset : field_offset (genv_cenv ge) SK._gfx
+    (co_members slide_node_co) = OK (0, Full);
+  slide_gfx_layout : (genv_cenv ge) ! SK._GraphNodeObject = Some slide_gfx_co;
+  slide_camera_offset : field_offset (genv_cenv ge) SK._cameraToObject
+    (co_members slide_gfx_co) = OK (84, Full)
+}.
+
+Definition slide_bindings (version : GameVersion) (ge : Clight.genv)
+    (animation animation_end sliding ground reflection action sound : block)
+    : Prop :=
+  Genv.find_symbol ge SK._set_mario_animation = Some animation /\
+  Genv.find_funct_ptr ge animation = Some (Internal (slide_animation_function version)) /\
+  Genv.find_symbol ge SK._is_anim_at_end = Some animation_end /\
+  Genv.find_funct_ptr ge animation_end = Some (Internal (slide_animation_end_function version)) /\
+  Genv.find_symbol ge SK._update_sliding = Some sliding /\
+  Genv.find_funct_ptr ge sliding = Some (Internal (slide_update_function version)) /\
+  Genv.find_symbol ge SK._perform_ground_step = Some ground /\
+  Genv.find_funct_ptr ge ground = Some (Internal (slide_ground_function version)) /\
+  Genv.find_symbol ge SK._mario_bonk_reflection = Some reflection /\
+  Genv.find_funct_ptr ge reflection = Some (Internal (slide_reflection_function version)) /\
+  Genv.find_symbol ge SK._set_mario_action = Some action /\
+  Genv.find_funct_ptr ge action = Some (Internal (slide_action_function version)) /\
+  Genv.find_symbol ge SK._play_sound = Some sound /\
+  Genv.find_funct_ptr ge sound = Some (Internal (slide_sound_function version)).
+
+(** The intermediate memories are ordered exactly as the generated caller.
+    m6 and m9 are its own star/dust assignments; the other changes belong to
+    the named callees, whose executions remain explicit. INPUT_OFF_FLOOR=4
+    is present at entry. This does not assume that the landing-dust body ran. *)
+Definition slide_helper_path (version : GameVersion) (ge : Clight.genv)
+    (m0 m1 m2 m3 m4 m5 m6 m7 m8 m9 : mem) (mario object : block) : Prop :=
+  Mem.load Mint16unsigned m0 mario 2 = Some (Vint (Int.repr 4)) /\
+  (exists animation_result,
+    eval_funcall function_entry2 ge m0 (Internal (slide_animation_function version))
+      [Vptr mario Ptrofs.zero; Vint (Int.repr 140)] E0 m1 animation_result) /\
+  eval_funcall function_entry2 ge m1 (Internal (slide_animation_end_function version))
+    [Vptr mario Ptrofs.zero] E0 m2 (Vint Int.zero) /\
+  (exists sliding_result,
+    eval_funcall function_entry2 ge m2 (Internal (slide_update_function version))
+      [Vptr mario Ptrofs.zero; Vsingle (Float32.of_bits (Int.repr 1065353216))]
+      E0 m3 sliding_result) /\
+  eval_funcall function_entry2 ge m3 (Internal (slide_ground_function version))
+    [Vptr mario Ptrofs.zero] E0 m4 (Vint (Int.repr 2)) /\
+  eval_funcall function_entry2 ge m4 (Internal (slide_reflection_function version))
+    [Vptr mario Ptrofs.zero; Vint Int.one] E0 m5 Vundef /\
+  Mem.load Mint32 m5 mario 8 = Some (Vint Int.zero) /\
+  Mem.store Mint32 m5 mario 8 (Vint (Int.repr 2)) = Some m6 /\
+  eval_funcall function_entry2 ge m6 (Internal (slide_action_function version))
+    [Vptr mario Ptrofs.zero; Vint (Int.repr 132194); Vint Int.zero]
+    E0 m7 (Vint Int.one) /\
+  Mem.load Mint32 m7 mario 20 = Some (Vint Int.zero) /\
+  Mem.load Mptr m7 mario 136 = Some (Vptr object Ptrofs.zero) /\
+  eval_funcall function_entry2 ge m7 (Internal (slide_sound_function version))
+    [Vint (Int.repr 335544321); Vptr object (Ptrofs.repr 84)] E0 m8 Vundef /\
+  Mem.load Mint32 m8 mario 8 = Some (Vint (Int.repr 2)) /\
+  Mem.store Mint32 m8 mario 8 (Vint (Int.repr 3)) = Some m9.
+
+Ltac slide_expr :=
+  first [solve [cog_expr] |
+    match goal with |- ?G => idtac "SLIDE EXPRESSION:" G end; fail 100].
+Ltac slide_check tac :=
+  first [solve [tac] |
+    match goal with |- ?G => idtac "SLIDE ATOMIC:" G end; fail 100].
+
+Ltac slide_stmt :=
+  lazymatch goal with
+  | |- exec_stmt _ _ _ _ _ Sskip _ _ _ _ => constructor
+  | |- exec_stmt _ _ _ _ _ Sbreak _ _ _ _ => constructor
+  | |- exec_stmt _ _ _ _ _ (Ssequence _ _) _ _ _ _ =>
+      first [eapply exec_Sseq_1 with (t1 := E0) (t2 := E0);
+             [slide_stmt | slide_stmt]
+            |eapply exec_Sseq_2; [slide_stmt | discriminate]]
+  | |- exec_stmt _ _ _ _ _ (Sset _ _) _ _ _ _ =>
+      eapply exec_Sset; slide_expr
+  | |- exec_stmt _ _ _ _ _ (Sassign _ _) _ _ _ _ =>
+      eapply exec_Sassign;
+      [cog_lvalue | slide_expr | cbn; reflexivity |
+       eapply assign_loc_value; [reflexivity | cbn; eassumption]]
+  | |- exec_stmt _ _ _ _ _ (Sifthenelse _ _ _) _ _ _ _ =>
+      eapply exec_Sifthenelse;
+      [slide_expr | cbn; reflexivity | cog_reduce_statement; slide_stmt]
+  | |- exec_stmt _ _ _ _ _ (Sswitch _ _) _ _ _ _ =>
+      eapply exec_Sswitch with (out := Out_break) (n := 2);
+      [slide_expr | cbn; reflexivity | cog_reduce_statement; slide_stmt]
+  | |- exec_stmt _ _ _ _ _ (Sreturn (Some _)) _ _ _ _ =>
+      eapply exec_Sreturn_some; slide_expr
+  | |- exec_stmt _ _ _ _ _ (Scall _ _ _) _ _ _ _ =>
+      eapply exec_Scall;
+      [reflexivity | slide_expr | slide_check cog_arguments |
+       slide_check ltac:(eapply cog_find_funct_zero; eassumption) |
+       reflexivity | slide_check ltac:(eassumption)]
+  end.
+
+Definition slide_kick_blocked_caller_claim (version : GameVersion) : Prop :=
+  forall (ge : Clight.genv) m0 m1 m2 m3 m4 m5 m6 m7 m8 m9 mario object
+      animation animation_end sliding ground reflection action sound,
+    slide_caller_layout ge ->
+    slide_bindings version ge animation animation_end sliding ground reflection action sound ->
+    slide_helper_path version ge m0 m1 m2 m3 m4 m5 m6 m7 m8 m9 mario object ->
+    eval_funcall function_entry2 ge m0 (Internal (slide_kick_function version))
+      [Vptr mario Ptrofs.zero] E0 m9 (Vint Int.zero) /\
+    Mem.load Mint32 m9 mario 8 = Some (Vint (Int.repr 3)).
+
+Theorem generated_slide_kick_blocked_caller_requests_dust_us_jp :
+  forall version, slide_kick_blocked_caller_claim version.
+Proof.
+  intros version ge m0 m1 m2 m3 m4 m5 m6 m7 m8 m9 mario object
+    animation animation_end sliding ground reflection action sound Hlayout Hbindings Hpath.
+  destruct Hlayout.
+  unfold slide_bindings in Hbindings. destruct Hbindings as
+    [Ha [Haf [He [Hef [Hu [Huf [Hg [Hgf [Hr [Hrf [Hac [Hacf [Hs Hsf]]]]]]]]]]]]].
+  unfold slide_helper_path in Hpath. destruct Hpath as
+    [Hinput [Hanimation [Hend [Hupdate [Hground [Hreflection [Hflags
+     [Hstars [Haction [Hterrain [Hobject [Hsound [Hstars_after Hdust]]]]]]]]]]]]].
+  destruct Hanimation as [animation_result Hanimation].
+  destruct Hupdate as [sliding_result Hupdate].
+  split.
+  - destruct version;
+      cbn [slide_kick_function slide_animation_function slide_animation_end_function
+        slide_update_function slide_ground_function slide_reflection_function
+        slide_action_function slide_sound_function] in *.
+    all: eapply eval_funcall_internal.
+    1,5: eapply function_entry2_intro;
+      [cbn; apply Coqlib.list_norepet_nil | cbn; cog_norepet |
+       vm_compute; intros x y Hx Hy Heq; subst y; intuition congruence |
+       cbn; apply alloc_variables_nil | cbn; reflexivity].
+    1,4: simpl fn_body; slide_stmt.
+    1,3: cbn; split; [discriminate | reflexivity].
+    all: cbn; reflexivity.
+  - rewrite (Mem.load_store_same _ _ _ _ _ _ Hdust). reflexivity.
+Qed.
+
+(** The numeric field offsets used above are checked against the generated
+    composite environment, independently in US and JP. *)
+Definition slide_generated_cenv (version : GameVersion) : composite_env :=
+  prog_comp_env
+    (match version with VersionUS => SK.prog
+                        | VersionJP => jp_mario_actions_moving.prog end).
+
+Definition slide_layout_offsets (version : GameVersion) : list (res (Z * bitfield)) :=
+  let ce := slide_generated_cenv version in
+  map (fun item => field_offset ce (snd item)
+    (match ce ! (fst item) with Some co => co_members co | None => [] end))
+    [(SK._MarioState,SK._input); (SK._MarioState,SK._particleFlags);
+     (SK._MarioState,SK._terrainSoundAddend); (SK._MarioState,SK._marioObj);
+     (SK._Object,SK._header); (SK._ObjectNode,SK._gfx);
+     (SK._GraphNodeObject,SK._cameraToObject);
+     (SK._MarioState,SK._pos); (SK._MarioState,SK._floor);
+     (SK._MarioState,SK._floorHeight)].
+
+Definition slide_layout_receipt : Prop :=
+  forall version, slide_layout_offsets version =
+    map (fun offset => OK (offset, Full)) [2;8;20;136;0;0;84;60;104;112].
+
+Theorem slide_caller_and_anchor_offsets_generated_us_jp : slide_layout_receipt.
+Proof. intros []; vm_compute; reflexivity. Qed.
+
+Definition slide_anchor (memory : mem) (mario : block) : list (option val) :=
+  [Mem.load Mfloat32 memory mario 60;
+   Mem.load Mfloat32 memory mario 64;
+   Mem.load Mfloat32 memory mario 68;
+   Mem.load Mptr memory mario 104;
+   Mem.load Mfloat32 memory mario 112].
+
+Lemma slide_particle_store_preserves_anchor :
+  forall before after mario flags,
+    Mem.store Mint32 before mario 8 (Vint flags) = Some after ->
+    slide_anchor after mario = slide_anchor before mario.
+Proof.
+  intros before after mario flags Hstore. unfold slide_anchor.
+  repeat rewrite (Mem.load_store_other _ _ _ _ _ _ Hstore)
+    by (right; right; cbn; lia).
+  reflexivity.
+Qed.
+
+(** This conditional frame rule covers the caller's seven callee boundaries
+    and its two own stores. It does not assert preservation INSIDE the
+    callee executions or across another game update. *)
+Definition slide_helpers_preserve_anchor mario m0 m1 m2 m3 m4 m5 m6 m7 m8 : Prop :=
+  slide_anchor m1 mario = slide_anchor m0 mario /\
+  slide_anchor m2 mario = slide_anchor m1 mario /\
+  slide_anchor m3 mario = slide_anchor m2 mario /\
+  slide_anchor m4 mario = slide_anchor m3 mario /\
+  slide_anchor m5 mario = slide_anchor m4 mario /\
+  slide_anchor m7 mario = slide_anchor m6 mario /\
+  slide_anchor m8 mario = slide_anchor m7 mario.
+
+Theorem slide_caller_own_stores_do_not_displace_mario :
+  forall version ge m0 m1 m2 m3 m4 m5 m6 m7 m8 m9 mario object,
+    slide_helper_path version ge m0 m1 m2 m3 m4 m5 m6 m7 m8 m9 mario object ->
+    slide_helpers_preserve_anchor mario m0 m1 m2 m3 m4 m5 m6 m7 m8 ->
+    map (fun m => slide_anchor m mario) [m0;m1;m2;m3;m4;m5;m6;m7;m8;m9] =
+      repeat (slide_anchor m0 mario) 10.
+Proof.
+  intros version ge m0 m1 m2 m3 m4 m5 m6 m7 m8 m9 mario object Hpath Hpreserve.
+  unfold slide_helper_path in Hpath. destruct Hpath as
+    [_ [_ [_ [_ [_ [_ [_ [Hstars [_ [_ [_ [_ [_ Hdust]]]]]]]]]]]]].
+  pose proof (slide_particle_store_preserves_anchor _ _ _ _ Hstars) as H6.
+  pose proof (slide_particle_store_preserves_anchor _ _ _ _ Hdust) as H9.
+  unfold slide_helpers_preserve_anchor in Hpreserve.
+  destruct Hpreserve as [H1 [H2 [H3 [H4 [H5 [H7 H8]]]]]].
+  cbn [map repeat]. congruence.
+Qed.
+
+Definition slide_kick_framed_caller_claim (version : GameVersion) : Prop :=
+  forall (ge : Clight.genv) m0 m1 m2 m3 m4 m5 m6 m7 m8 m9 mario object
+      animation animation_end sliding ground reflection action sound,
+    slide_caller_layout ge ->
+    slide_bindings version ge animation animation_end sliding ground reflection action sound ->
+    slide_helper_path version ge m0 m1 m2 m3 m4 m5 m6 m7 m8 m9 mario object ->
+    slide_helpers_preserve_anchor mario m0 m1 m2 m3 m4 m5 m6 m7 m8 ->
+    eval_funcall function_entry2 ge m0 (Internal (slide_kick_function version))
+      [Vptr mario Ptrofs.zero] E0 m9 (Vint Int.zero) /\
+    Mem.load Mint32 m9 mario 8 = Some (Vint (Int.repr 3)) /\
+    map (fun m => slide_anchor m mario) [m0;m1;m2;m3;m4;m5;m6;m7;m8;m9] =
+      repeat (slide_anchor m0 mario) 10.
+
+Theorem generated_slide_kick_dust_caller_with_anchor_boundaries_us_jp :
+  forall version, slide_kick_framed_caller_claim version.
+Proof.
+  intros version ge m0 m1 m2 m3 m4 m5 m6 m7 m8 m9 mario object
+    animation animation_end sliding ground reflection action sound
+    Hlayout Hbindings Hpath Hanchors.
+  destruct (generated_slide_kick_blocked_caller_requests_dust_us_jp version
+    ge m0 m1 m2 m3 m4 m5 m6 m7 m8 m9 mario object
+    animation animation_end sliding ground reflection action sound
+    Hlayout Hbindings Hpath) as [Hcall Hflags].
+  refine (conj Hcall (conj Hflags _)).
+  eapply slide_caller_own_stores_do_not_displace_mario;
+    [exact Hpath | exact Hanchors].
+Qed.
